relabel/relabel.v
@@ -30,12 +30,12 @@ Fixpoint labelPost {X} (t: Tree X) (t_res : Tree ident) : iProp :=
   | _, _ => False
   end.
 
-Lemma label_spec : forall X (tree : Tree X),
-    ⊢ {{ emp }} label tree {{ tree'; labelPost tree tree' }}.
+Lemma label_spec : forall X (t : Tree X),
+    ⊢ {{ emp }} label t {{ t'; labelPost t t' }}.
 Proof.
-  induction tree.
+  induction t.
   - iBind. eapply gensym_spec. iRet.
-  - iBind. eapply IHtree1. iBind. Frame. eapply IHtree2. iRet. iIntros "[$ $]".
+  - iBind. eapply IHt1. iBind. Frame. eapply IHt2. iRet. iIntros "[$ $]".
 Qed.
 
 Fixpoint flatten {X} (t: Tree X) : list X :=
@@ -51,11 +51,11 @@ Definition sameShape {X Y} (t1 : Tree X) (t2 : Tree Y) : Prop :=
   | _, _ => False
   end.
 
-Lemma labelpost_fold : forall X (tree : Tree X) tree0,
-    ⊢ labelPost tree tree0 -∗ [∗ list] x ∈ (flatten tree0), IsFresh x.
+Lemma labelpost_fold : forall X (t : Tree X) t',
+    ⊢ labelPost t t' -∗ [∗ list] x ∈ (flatten t'), IsFresh x.
 Proof.
-  induction tree, tree0; simpl; iIntros; norm_all; auto; try contradiction.
-  iDestruct (IHtree1 with "HB") as "Ht1". iDestruct (IHtree2 with "HC") as "Ht2".
+  induction t, t'; simpl; iIntros; norm_all; auto; try contradiction.
+  iDestruct (IHt1 with "HB") as "Ht1". iDestruct (IHt2 with "HC") as "Ht2".
   iApply big_sepL_app. iFrame.
 Qed.
 
@@ -64,10 +64,9 @@ Proof.
   induction l; iIntros "* HA HB".
   - iPureIntro. intro. inversion H.
   - iDestruct "HB" as "[HA' HB]".
-    destruct (eq_dec a a0).
-    + iExFalso. subst. iApply (singleton_false with "HA HA'").
-    + iDestruct (IHl with "HA HB") as "%". iPureIntro.
-      intro. inversion H0; subst; auto.
+    iDestruct (singleton_neq with "HA HA'") as "%".
+    iDestruct (IHl with "HA HB") as "%". iPureIntro.
+    intro. inversion H1; subst; auto.
 Qed.
 
 Lemma fold_nodup : forall l,
@@ -86,17 +85,17 @@ Proof.
   iDestruct (fold_nodup with "HB") as "$".
 Qed.
 
-Lemma finish_him : forall X (tree : Tree X) tree0 h,
-    labelPost tree tree0 () h -> NoDup (flatten tree0) /\ sameShape tree tree0.
+Lemma finish_him : forall X (t : Tree X) t' h,
+    labelPost t t' () h -> NoDup (flatten t') /\ sameShape t t'.
 Proof.
   intros. apply soundness3 in H. apply (soundness1 h).
   iIntros "HA". iDestruct (H with "HA") as "HA". iDestruct (labelpost_nodup with "HA") as "%".
-  iSplit; auto. destruct tree,tree0; auto.
+  iSplit; auto. destruct t,t'; auto.
 Qed.
 
-Lemma relabel_spec : forall X (tree : Tree X) tree0,
-    relabel tree = tree0 -> NoDup (flatten tree0) /\ sameShape tree tree0.
+Lemma relabel_spec : forall X (t : Tree X) t',
+    relabel t = t' -> NoDup (flatten t') /\ sameShape t t'.
 Proof.
-  intros. unfold relabel in H. destruct (run (label tree) initial_state) eqn:?. destruct H. simpl.
-  eapply (finish_him _ _ _ _ (adequacy_triple_init _ _ _ _ _ emp_trivial (label_spec _ tree) Heqp)).
+  intros. unfold relabel in H. destruct (run (label t) initial_state) eqn:?. destruct H. simpl.
+  eapply (finish_him _ _ _ _ (adequacy_triple_init _ _ _ _ _ emp_trivial (label_spec _ t) Heqp)).
 Qed.
